coq/theories/imperative/ImpSemantics.v
@@ -6,37 +6,6 @@ Require Import impboot.imperative.ImpSyntax.
 Require Import coqutil.Word.Interface.
 Require Import coqutil.Word.Properties.
 
-(* monadic *)
-
-Inductive Monadic {M: Type -> Type} : Type -> Type :=
-| Pure {A: Type} (a: A): Monadic A
-| Bind {A B: Type} (ma: Monadic A) (f: A -> Monadic B): Monadic B
-| Lift {A: Type} (ma: M A): Monadic A.
-Arguments Monadic: clear implicits.
-
-Definition bind {M: Type -> Type} {A B : Type} (ma: Monadic M A) (f: A -> Monadic M B): Monadic M B :=
-  Bind ma f.
-
-Definition map {M: Type -> Type} {A B : Type} (ma: Monadic M A) (f: A -> B): Monadic M B :=
-  Bind ma (fun a => Pure (f a)).
-
-Definition point {M: Type -> Type} {A : Type} (a : A) : Monadic M A :=
-  Pure a.
-
-Definition lift {M: Type -> Type} {A: Type} (ma: M A): Monadic M A :=
-  Lift(ma).
-
-Notation "'let+' v := r1 'in' r2" :=
-  (bind r1 (fun v => r2))
-  (at level 200, right associativity).
-
-Notation "'let+' ( v1 , v2 ) := r1 'in' r2" :=
-  (bind r1 (fun v => let (v1, v2) := v in r2))
-  (at level 200, right associativity).
-
-Notation "r1 ;; r2" := (let+ _ := r1 in r2)
-  (at level 200, right associativity).
-
 (* types *)
 
 Notation mem_block := (list (option Value)) (only parsing).
@@ -49,72 +18,65 @@ Record state := mkState {
   output: list ascii
 }.
 
-Inductive outV :=
-| Return (v: Value)
+Inductive result {A : Type} :=
+| Return (v: A)
 | TimeOut
 | Crash
 | Abort.
-Arguments outV : clear implicits.
-
-Inductive result {A : Type} :=
-| Interm (v: A)
-| Stop (v: outV)
-| ContDF (c: cmd) (cnt: Monadic (fun a => state -> (@result a * state)) A).
 Arguments result : clear implicits.
+
+Inductive outcome {A B : Type} :=
+| Cont (v: B)
+| Stop (v: result A).
+Arguments outcome : clear implicits.
 
 (* monad syntax *)
 
-Notation ResM A := (result A * state)%type (only parsing).
-Notation StateResM A := (state -> (result A * state))%type (only parsing).
+Notation MRes A := (outcome Value A * state)%type (only parsing).
+Notation M A := (state -> MRes A) (only parsing).
 
-Definition bindM {A B : Type} (ma: StateResM A) (f: A -> StateResM B): StateResM B :=
+Definition bind {A B : Type} (ma: M A) (f: A -> M B): M B :=
   (fun s =>
     match ma s with
-    | (Interm res, s1) => f res s1
+    | (Cont res, s1) => f res s1
     | (Stop e, s1) => (Stop e, s1)
-    (* ContDF not allowed here *)
-    | (ContDF c cnt, s1) => (Stop Crash, s1)
     end
   ).
 
-Definition mapM {A B : Type} (ma: StateResM A) (f: A -> B): StateResM B :=
-  (fun s =>
-    match ma s with
-    | (Interm res, s1) => (Interm (f res), s1)
-    | (Stop e, s1) => (Stop e, s1)
-    (* ContDF not allowed here *)
-    | (ContDF c cnt, s1) => (Stop Crash, s1)
-    end
-  ).
+Definition bindMRes {A B : Type} (ma: MRes A) (f: A -> state -> MRes B): MRes B :=
+  match ma with
+  | (Cont res, s1) => f res s1
+  | (Stop e, s1) => (Stop e, s1)
+  end.
 
-Definition pointM {A : Type} (a : A) : StateResM A :=
-  (fun s => (Interm a, s)).
+Definition point {A : Type} (a : A) : M A :=
+  (fun s => (Cont a, s)).
 
-Notation "'letM+' v := r1 'in' r2" :=
-  (bindM r1 (fun v => r2))
+Notation "'let+' v := r1 'in' r2" :=
+  (bind r1 (fun v => r2))
   (at level 200, right associativity).
 
-Notation "'letM+' ( v1 , v2 ) := r1 'in' r2" :=
-  (bindM r1 (fun v => let (v1, v2) := v in r2))
+Notation "'let+' ( v1 , v2 ) := r1 'in' r2" :=
+  (bind r1 (fun v => let (v1, v2) := v in r2))
   (at level 200, right associativity).
 
-Notation SRM A := (Monadic (fun a => state -> (result a * state)) A) (only parsing).
+Notation "'let*' ( v , s ) := r1 'in' r2" :=
+  (bindMRes r1 (fun v s => r2)) (at level 200, right associativity).
 
-Definition stop {B} (v : outV) (s : state) : (result B * state) :=
+Notation "r1 ;; r2" := (let+ _ := r1 in r2)
+  (at level 200, right associativity).
+
+Definition stop {A B} (v : result A) (s : state) : (outcome A B * state) :=
   (Stop v, s).
-Arguments stop _ !v !s /.
+Arguments stop _ _ !v !s /.
 
-Definition crash {B} (s : state) : (result B * state) :=
+Definition crash {A B} (s : state) : (outcome A B * state) :=
   stop Crash s.
-Arguments crash _ !s /.
+Arguments crash _ _ !s /.
 
-Definition interm {B} (v : B) (s : state) : (result B * state) :=
-  (Interm v, s).
-Arguments interm _ !v !s /.
-
-Definition contdf {B} (c : cmd) (cnt: SRM B) (s : state) : (result B * state) :=
-  (ContDF c cnt, s).
-Arguments contdf _ !c !cnt !s /.
+Definition cont {A B} (v : B) (s : state) : (outcome A B * state) :=
+  (Cont v, s).
+Arguments cont _ _ !v !s /.
 
 Definition next (input : llist ascii) : Value :=
   match input with
@@ -122,19 +84,19 @@ Definition next (input : llist ascii) : Value :=
   | Lcons c cs => Word (word.of_Z (Z.of_nat (nat_of_ascii c)))
   end.
 
-Definition lookup_var (n : name) (s : state) : ResM Value :=
+Definition lookup_var (n : name) (s : state) : MRes Value :=
   match IEnv.lookup s.(vars) n with
-  | Some v => interm v s
+  | Some v => cont v s
   | None => crash s
   end.
 
-Definition combine_word (f : word64 -> word64 -> word64) (x y : Value): StateResM Value :=
+Definition combine_word (f : word64 -> word64 -> word64) (x y : Value): M Value :=
   match x, y with
-  | Word w1, Word w2 => interm (Word (f w1 w2))
+  | Word w1, Word w2 => cont (Word (f w1 w2))
   | _, _ => stop Crash
   end.
 
-Definition mem_load (ptr val : Value) (s : state) : (result Value * state) :=
+Definition mem_load (ptr val : Value) (s : state) : (outcome Value Value * state) :=
   match ptr, val with
   | Pointer p, Word w =>
     if negb (((w2n w) mod 8) =? 0) then crash s else
@@ -143,7 +105,7 @@ Definition mem_load (ptr val : Value) (s : state) : (result Value * state) :=
     | Some block =>
       let idx := (w2n w) / 8 in
       match List.nth_error block idx with
-      | Some (Some w) => interm w s
+      | Some (Some w) => cont w s
       | _ => crash s
       end
     end
@@ -185,32 +147,32 @@ Definition set_fuel (fuel: nat) (s: state) : state :=
      input := s.(input);
      output := s.(output) |}.
 
-Fixpoint eval_exp (e : exp) : StateResM Value :=
+Fixpoint eval_exp (e : exp) : M Value :=
   match e with
   | Var n => lookup_var n
-  | Const n => interm (Word n)
+  | Const n => cont (Word n)
   | Add e1 e2 =>
-      letM+ v1 := eval_exp e1 in
-      letM+ v2 := eval_exp e2 in
+      let+ v1 := eval_exp e1 in
+      let+ v2 := eval_exp e2 in
       combine_word word.add v1 v2
   | Sub e1 e2 =>
-      letM+ v1 := eval_exp e1 in
-      letM+ v2 := eval_exp e2 in
+      let+ v1 := eval_exp e1 in
+      let+ v2 := eval_exp e2 in
       combine_word word.sub v1 v2
   | Div e1 e2 =>
-      letM+ v1 := eval_exp e1 in
-      letM+ v2 := eval_exp e2 in
+      let+ v1 := eval_exp e1 in
+      let+ v2 := eval_exp e2 in
       if value_eqb v2 (Word (word.of_Z 0))
       then crash
       else combine_word word.divu v1 v2
   | Read e1 e2 =>
-      letM+ addr := eval_exp e1 in
-      letM+ offset := eval_exp e2 in
+      let+ addr := eval_exp e1 in
+      let+ offset := eval_exp e2 in
       mem_load addr offset
   end.
 
 Ltac unfold_monadic :=
-  unfold interm, crash, stop, pointM, bindM, point, bind, combine_word, mem_load in *.
+  unfold cont, crash, stop, point, bind, combine_word, mem_load in *.
 
 Ltac crunch_monadic :=
   repeat match goal with
@@ -231,13 +193,13 @@ Proof.
   all: crunch_monadic; eapply IHe1 in Heqp; try eapply IHe2 in Heqp0; congruence.
 Qed.
 
-Fixpoint eval_exps (es : list exp) : StateResM (list Value) :=
+Fixpoint eval_exps (es : list exp) : M (list Value) :=
   match es with
-  | [] => interm []
+  | [] => cont []
   | e :: es =>
-    letM+ v := eval_exp e in
-    letM+ vs := eval_exps es in
-    interm (v :: vs)
+    let+ v := eval_exp e in
+    let+ vs := eval_exps es in
+    cont (v :: vs)
   end.
 
 Theorem eval_exps_pure: forall (es: list exp) r (s s': state),
@@ -248,23 +210,23 @@ Proof.
   - crunch_monadic; try eapply eval_exp_pure in Heqp; try eapply IHes in Heqp0; congruence.
 Qed.
 
-Definition dest_word (v: Value) : StateResM word64 :=
+Definition dest_word (v: Value) : M word64 :=
   match v with
-  | Word w => interm w
+  | Word w => cont w
   | _ => crash
   end.
 
-Definition eval_cmp (c: cmp) (v1 v2: Value): StateResM bool :=
+Definition eval_cmp (c: cmp) (v1 v2: Value): M bool :=
   match c, v1, v2 with
   | Less, Word w1, Word w2 =>
-    interm (w1 <w w2)
+    cont (w1 <w w2)
   | Equal, Word w1, Word w2 =>
-    interm (w1 =w w2)
+    cont (w1 =w w2)
   (* TODO(kπ) Ask Magnus or Clement? I removed this. Dunno how to distinguish
   pointer vs word in asm. *)
   (* assume that every allocated address is greater than zero *)
   (* | Equal, Pointer p, Word w =>
-    (if w =w (word.of_Z 0) then interm false else stop Crash) *)
+    (if w =w (word.of_Z 0) then cont false else stop Crash) *)
   | _, _, _ => stop Crash
   end.
 
@@ -274,23 +236,23 @@ Proof.
   destruct c; simpl; intros; crunch_monadic; try congruence.
 Qed.
 
-Fixpoint eval_test (t : test) : StateResM bool :=
+Fixpoint eval_test (t : test) : M bool :=
   match t with
   | Test c e1 e2 =>
-      letM+ v1 := eval_exp e1 in
-      letM+ v2 := eval_exp e2 in
+      let+ v1 := eval_exp e1 in
+      let+ v2 := eval_exp e2 in
       eval_cmp c v1 v2
   | And t1 t2 =>
-    letM+ v1 := eval_test t1 in
-    letM+ v2 := eval_test t2 in
-    interm (andb v1 v2)
+    let+ v1 := eval_test t1 in
+    let+ v2 := eval_test t2 in
+    cont (andb v1 v2)
   | Or t1 t2 =>
-    letM+ v1 := eval_test t1 in
-    letM+ v2 := eval_test t2 in
-    interm (orb v1 v2)
+    let+ v1 := eval_test t1 in
+    let+ v2 := eval_test t2 in
+    cont (orb v1 v2)
   | Not t =>
-    letM+ v := eval_test t in
-    interm (negb v)
+    let+ v := eval_test t in
+    cont (negb v)
   end.
 
 Theorem eval_test_pure: forall (t: test) r (s s': state),
@@ -302,8 +264,8 @@ Proof.
   crunch_monadic; eapply IHt in Heqp; congruence.
 Qed.
 
-Definition assign (n: name) (v : Value) (s : state) : ResM unit :=
-  interm tt (set_vars (IEnv.insert (n, Some v) s.(vars)) s).
+Definition assign (n: name) (v : Value) (s : state) : MRes unit :=
+  cont tt (set_vars (IEnv.insert (n, Some v) s.(vars)) s).
 
 Fixpoint find_fun (fname : name) (fs : list func): option (list name * cmd) :=
   match fs with
@@ -315,7 +277,7 @@ Fixpoint find_fun (fname : name) (fs : list func): option (list name * cmd) :=
 Definition update_block (vs:mem_block) offset v : option mem_block :=
   if offset <? List.length vs then Some (list_update offset (Some v) vs) else None.
 
-Definition update (v1 v2 v : Value) (s: state): ResM unit :=
+Definition update (v1 v2 v : Value) (s: state): MRes unit :=
   match v1, v2 with
   | (Pointer p), (Word offset) =>
     if negb ((w2n offset) mod 8 =? 0) then crash s else
@@ -324,190 +286,131 @@ Definition update (v1 v2 v : Value) (s: state): ResM unit :=
       | Some vs =>
         match update_block vs ((w2n offset) / 8) v with
         | None => crash s
-        | Some ws => interm tt (set_memory (list_update p ws s.(memory)) s)
+        | Some ws => cont tt (set_memory (list_update p ws s.(memory)) s)
         end
       end
   | _, _ => crash s
   end.
 
-Definition alloc (len: word64) (s: state) : ResM Value :=
+Definition alloc (len: word64) (s: state) : MRes Value :=
   if negb ((w2n len) mod 8 =? 0) then crash s else
-    interm (Pointer (List.length s.(memory)))
+    cont (Pointer (List.length s.(memory)))
       (set_memory (s.(memory) ++ [repeat None ((w2n len) / 8)]) s).
 
-Definition put_char (v: Value) (s: state): ResM unit :=
+Definition put_char (v: Value) (s: state): MRes unit :=
   match v with
   | (Pointer p) => crash s
   | (Word w) =>
     if w2n w <? 256 then
-      interm tt (set_output (s.(output) ++ [ascii_of_nat (w2n w)]) s)
+      cont tt (set_output (s.(output) ++ [ascii_of_nat (w2n w)]) s)
     else crash s
   end.
 
-Definition get_char (s: state) : ResM Value :=
-  interm (next s.(input))
+Definition get_char (s: state) : MRes Value :=
+  cont (next s.(input))
     (set_input (Llist.ltail s.(input)) s).
 
-Definition get_vars (s: state): ResM IEnv.env :=
-  interm s.(vars) s.
+Definition get_vars (s: state): MRes IEnv.env :=
+  cont s.(vars) s.
 
-Definition set_varsM (vars: IEnv.env) (s: state): ResM unit :=
-  interm tt (set_vars vars s).
+Definition set_varsM (vars: IEnv.env) (s: state): MRes unit :=
+  cont tt (set_vars vars s).
 
 Definition nodupb (l: list nat): bool :=
   if NoDup_dec Nat.eq_dec l then
     true
   else false.
 
-Definition get_body_and_set_vars (nm: name) (vs: list Value) (s: state): ResM cmd :=
+Definition get_body_and_set_vars (nm: name) (vs: list Value) (s: state): MRes cmd :=
   match find_fun nm s.(funs) with
   | None => crash s
   | Some (params, body) =>
       if orb (negb (List.length params =? List.length vs)) (negb (nodupb params)) then
         crash s
       else
-        interm body (set_vars (IEnv.insert_all (List.combine params (List.map Some vs)) IEnv.empty) s)
+        cont body (set_vars (IEnv.insert_all (List.combine params (List.map Some vs)) IEnv.empty) s)
   end.
 
-Definition catch_return {A} (f: StateResM A) (s: state): ResM Value :=
+Definition catch_return {A} (f: M A) (s: state): MRes Value :=
     match f s with
-    | (Interm _, s) => crash s
-    | (Stop (Return v), s) => interm v s
+    | (Cont _, s) => crash s
+    | (Stop (Return v), s) => cont v s
     | (Stop TimeOut,s) => stop TimeOut s
     | (Stop Crash,s) => stop Crash s
     | (Stop Abort,s) => stop Abort s
-    (* TODO(kπ) *)
-    | (ContDF c cnt, s) =>
-      stop Crash s
-      (* (ContDF c cnt, s) *)
   end.
 
-Fixpoint eval_cmd (c: cmd) { struct c } : SRM unit :=
+Fixpoint eval_cmd (c : cmd)
+  (EVAL_CMD : forall (c:cmd), M unit)
+  { struct c } : M unit :=
+  let eval_cmd c := eval_cmd c EVAL_CMD in
   match c with
   | Seq c1 c2 =>
     let+ _ := eval_cmd c1 in
     eval_cmd c2
   | Assign n e =>
-    let+ v := lift (eval_exp e) in
-    lift (assign n v)
-  | ImpSyntax.Abort => lift (stop Abort)
+    let+ v := eval_exp e in
+    assign n v
+  | ImpSyntax.Abort => stop Abort
   | PutChar e =>
-    let+ v := lift (eval_exp e) in
-    lift (put_char v)
+    let+ v := eval_exp e in
+    put_char v
   | GetChar n =>
-    let+ v := lift get_char in
-    lift (assign n v)
+    let+ v := get_char in
+    assign n v
   | Alloc n e =>
-    let+ val := lift (eval_exp e) in
-    let+ len := lift (dest_word val) in
-    let+ ptr := lift (alloc len) in
-    lift (assign n ptr)
+    let+ val := eval_exp e in
+    let+ len := dest_word val in
+    let+ ptr := alloc len in
+    assign n ptr
   | Update a e e' =>
-    let+ ptr := lift (eval_exp a) in
-    let+ off := lift (eval_exp e) in
-    let+ val := lift (eval_exp e') in
-    lift (update ptr off val)
+    let+ ptr := eval_exp a in
+    let+ off := eval_exp e in
+    let+ val := eval_exp e' in
+    update ptr off val
   | If t c1 c2 =>
-    let+ cond := lift (eval_test t) in
-    if (cond: bool)
+    let+ cond := eval_test t in
+    if cond
     then eval_cmd c1
     else eval_cmd c2
   | ImpSyntax.Return e =>
-    let+ v := lift (eval_exp e) in
-    lift (stop (Return v))
+    let+ v := eval_exp e in
+    stop (Return v)
   | While t c =>
-    let+ cond := lift (eval_test t) in
-    if (cond: bool) then
+    let+ cond := eval_test t in
+    if cond then
       let+ _ := (eval_cmd c) in
-      lift (contdf (While t c) (lift (interm tt)))
+      (EVAL_CMD (While t c))
     else
-      lift (interm tt)
+      cont tt
   | Call n fname es =>
-    lift (interm tt)
-    (* TODO(kπ) *)
-    (* let+ vs := lift (eval_exps es) in
-    let+ vars := lift get_vars in
-    let+ body := lift (get_body_and_set_vars fname vs) in
-    let+ v := catch_return (contdf body) in
-    let+ _ := lift (assign n v) in
-    set_varsM vars *)
+    let+ vs := eval_exps es in
+    let+ vars := get_vars in
+    let+ body := get_body_and_set_vars fname vs in
+    let+ v := catch_return (EVAL_CMD body) in
+    let+ _ := assign n v in
+    set_varsM vars
   end.
 
-Fixpoint interp {A} (m : SRM A) (s : state) : (result A * state) :=
-  match m with
-  | Pure a => (Interm a, s)
-  | Bind ma f =>
-      match interp ma s with
-      | (Interm a, s') => interp (f a) s'
-      | (Stop v, s') => (Stop v, s')
-      (* vvv This loses the info from upper calls *)
-      | (ContDF c cnt, s') => (ContDF c (Bind cnt f), s')
-      end
-  | Lift ma => ma s
-  end.
-
-Program Fixpoint EVAL_CMD (fuel: nat) (c : SRM unit) {measure fuel} : state -> ((result unit * state) * nat)%type :=
-  fun s =>
-    match fuel with
-    | 0 => (stop TimeOut s, 0)
-    | S fuel =>
-      match interp c s with
-      | (Interm v, s1) => (interm v s1, S fuel)
-      | (Stop out, s1) => (stop out s1, S fuel)
-      | (ContDF c1 cnt, s1) =>
-          let (r, fuel1) := EVAL_CMD fuel (eval_cmd c1) s1 in
-          EVAL_CMD fuel1 cnt s1
-      end
-    end.
-
-(* Fixpoint EVAL_CMD (fuel: nat) (c : cmd) {struct fuel} : state -> ((result unit * state) * nat)%type :=
-  fun s =>
+Fixpoint EVAL_CMD (fuel: nat) (c : cmd) {struct fuel} : M unit :=
   match fuel with
-  | 0 => (stop TimeOut s, 0)
-  | S fuel =>
-    match eval_cmd c s with
-    | (Interm v, s) => (interm v s, S fuel)
-    | (Stop out, s) => (stop out s, S fuel)
-    | (ContDF c cnt, s) =>
-      let r := EVAL_CMD fuel c s in (* might give smaller fuel as a result *)
-      match r with
-      | ((Stop (Return v), s1), fuel1) => (cnt (Some v) s1, fuel1)
-      | ((_, s1), fuel1) => (cnt None s1, fuel1)
-      end
-    end
-  end. *)
+  | 0 => stop TimeOut
+  | S fuel => eval_cmd c (EVAL_CMD (fuel - 1))
+  end.
 
-Definition init_state (inp: llist ascii) (funs: list func): state :=
+Definition init_state (inp: llist ascii) (funs: list func) (fuel: nat): state :=
   {| vars   := IEnv.empty;
      memory := [];
      funs   := funs;
      input  := inp;
      output := []; |}.
 
-Definition example_program :=
-  Seq
-    (Seq
-      (Assign 0 (Const (word.of_Z 0))) (* i := 0 *)
-      (Seq
-        (While (Test Less (Var 0) (Const (word.of_Z 5))) (* i < 5 *)
-          (Assign 0 (Add (Var 0) (Const (word.of_Z 1))))) (* i = i + 1 *)
-        (Assign 0 (Const (word.of_Z 42))) (* x := 42 *)
-      ))
-    (PutChar (Const (word.of_Z 65))). (* putchar 'A' *)
-
-Compute (
-  let (rs, f) := EVAL_CMD 10 example_program (init_state Lnil []) in
-  let (r, s) := rs in
-  s.(vars) 0
-).
-
-Definition eval_from (fuel: nat) (input: llist ascii) (p: prog): ResM unit :=
+Definition eval_from (fuel: nat) (input: llist ascii) (p: prog): MRes unit :=
   match p with
   | Program funs =>
     let call_main_cmd: cmd := (Call 0 (name_of_string "main") []) in
-    let init_s := init_state input funs in
-    let (res, fuel1) := EVAL_CMD fuel call_main_cmd init_s in
-    res
+    let init_s := init_state input funs fuel in
+    eval_cmd call_main_cmd (EVAL_CMD fuel) init_s
   end.
 
 Definition imp_avoids_crash (input: llist ascii) (p: prog) :=
@@ -526,6 +429,6 @@ Definition imp_output (fuel: nat) (input: llist ascii) (p: prog) :=
     output = build_lprefix_lub { imp_output fuel input p | k IN UNIV }. *)
 
 Definition imp_weak_termination (input: llist ascii) (p: prog) (out: list ascii) :=
-  exists fuel result s,
-    eval_from fuel input p = (result, s) /\
-    (result <> Stop Abort -> result = Interm tt /\ s.(output) = out).
+  exists fuel outcome s,
+    eval_from fuel input p = (outcome, s) /\
+    (outcome <> Stop Abort -> outcome = Cont tt /\ s.(output) = out).
